Prove init_at correct
Relies on knowing sizes are equal and establishes that the contents are
equal. Init will check that sizes are equal and then call init_at.

src/SeqDisk/ReplicatedDisk/Init.v
@@ -44,4 +44,88 @@ Section Init.
                    end
       end.
 
+  Lemma le_eq_or_S_le : forall n m,
+      n <= m ->
+      n = m \/
+      S n <= m /\ n <> m.
+  Proof.
+    inversion 1; eauto.
+    right; intuition eauto using le_n_S.
+    subst.
+    eapply PeanoNat.Nat.nle_succ_diag_l; eauto.
+  Qed.
+
+  Definition equal_after a (d_0 d_1: disk) :=
+    size d_0 = size d_1 /\
+    forall a', a <= a' -> d_0 a' = d_1 a'.
+
+  Lemma equal_after_diskUpd : forall a d_0 d_1 b,
+      equal_after (S a) d_0 d_1 ->
+      equal_after a (diskUpd d_0 a b) (diskUpd d_1 a b).
+  Proof.
+    unfold equal_after; intuition.
+    autorewrite with upd; eauto.
+    apply le_eq_or_S_le in H; intuition subst.
+    destruct (lt_dec a' (size d_0)); autorewrite with upd.
+    assert (a' < size d_1) by congruence; autorewrite with upd; auto.
+    assert (~a' < size d_1) by congruence; autorewrite with upd; auto.
+    autorewrite with upd; eauto.
+  Qed.
+
+  Hint Resolve equal_after_diskUpd.
+
+  Theorem init_at_ok : forall a,
+      prog_spec
+        (fun '(d_0, d_1) state =>
+           {| pre :=
+                TD.disk0 state |= eq d_0 /\
+                TD.disk1 state |= eq d_1 /\
+                equal_after a d_0 d_1;
+              post :=
+                fun _ state' =>
+                  exists d_0' d_1',
+                    TD.disk0 state' |= eq d_0' /\
+                    TD.disk1 state' |= eq d_1' /\
+                    equal_after 0 d_0' d_1';
+              recover :=
+                fun _ state' => True;
+           |})
+        (init_at a)
+        (irec td)
+        (refinement td).
+  Proof.
+    induction a; simpl; intros.
+    - step.
+    - step.
+      descend; intuition eauto.
+
+      step.
+      destruct r.
+      + descend; intuition eauto.
+        step.
+        destruct r.
+        descend; intuition eauto.
+
+        simplify.
+        descend; intuition eauto.
+      + descend; intuition eauto.
+        step.
+        destruct r; simplify.
+        descend; intuition eauto; simplify.
+        descend; (intuition eauto); simplify.
+
+        Grab Existential Variables.
+        exact block0.
+  Qed.
+
+  Lemma equal_after_0_to_eq : forall d_0 d_1,
+      equal_after 0 d_0 d_1 ->
+      d_0 = d_1.
+  Proof.
+    unfold equal_after; intuition.
+    eapply diskMem_ext_eq.
+    extensionality a'.
+    eauto using le_0_n.
+  Qed.
+
 End Init.
